\documentclass[12pt]{article}

\date{December 31 2019}
\title{$(1 \cong 0) \cong (1 \land 0 \land 0_{XY} \forall X, Y \in Ob(C))$}
\usepackage{amsmath}

\begin{document}

\maketitle

\begin{equation}
\tag{to}
\begin{aligned}
& (1 \cong 0) \Rightarrow \\
& \forall X, Y \in Ob(C)\; \exists! 1^{X} \in X \rightarrow 1 \land \\
& \exists! Y^{0} \in 0 \rightarrow Y \Rightarrow \\
& \exists! 0_{XY} \in X \rightarrow Y = Y^{0} \cdot 0^{1} \cdot 1^{X}
\end{aligned}
\end{equation}

\begin{equation}
\tag{from}
\begin{aligned}
& (1 \land 0 \land 0_{XY} \forall X, Y \in Ob(C)) \Rightarrow \\
& (\forall X, Y \in Ob(C) \exists! 0_{XY} \in X \rightarrow Y \Rightarrow \\
& (0_{10} \in 1 \rightarrow 0 \land \\
& \forall Z \in Ob(C) \exists! Z^{0} \in 0 \rightarrow Z \land \\
& \forall Q \in Ob(C) \exists! 1^{Q} \in Q \rightarrow 1) \Rightarrow \\
& 0_{10} \cdot 1^{0} = 0^{0} = 1_{0} \land \\
& 1^{0} \cdot 0_{10} = 1^{1} = 1_{1} \Rightarrow \\
& (1 \cong 0)
\end{aligned}
\end{equation}

\end{document}
