\documentclass[fleqn, 11pt]{article}

\date{January 13, 2020}
\pagestyle{empty}
\title{DeMorgan's Laws}
\usepackage{amsmath}
\usepackage{amssymb}
\usepackage{mathtools}

\begin{document}

$$ \forall n \in \mathbb{N+}; \; B - \cap (A_1 .. A_n) = \cup((B - A_1) .. (B - A_n)) $$
\begin{equation*}
\begin{aligned}
& \\
& n = 1 \Rightarrow B - (A_1 \cap A_1) = B - A_1 = (B - A_1) \cup (B - A_1) \\
& \\
& n = 2 \Rightarrow B - (A_1 \cap A_2) =  \\
& \qquad \{x \mid x \in B \land x \in \{y \mid y \in A_1 \land y \in A_2 \}\} = \\
& \qquad \{x \mid x \in B \land (x \notin A_1 \lor x \notin A_2)\} = \\
& \qquad (B - A_1) \cup (B - A_2) \\
& \\
& n = k + 1 \Rightarrow B - \cap(A_1 .. A_{k+1}) = & (assoc \; \cap) \\
& \qquad B - (\cap(A_1 .. A_k) \cap A_{k+1}) = & (n = 2) \\
& \qquad (B - \cap(A_1 ..A_k)) \cup (B - A_{k+1}) = & (ind. \; hyp.) \\
& \qquad \cup((B - A_1) .. (B - A_k)) \cup (B - A_{k+1}) = & (assoc \; \cup) \\
& \qquad \cup((B - A_1) .. (B - A_{k+1})) \\
& \blacksquare
\end{aligned}
\end{equation*}

$$ \forall n \in \mathbb{N+}; \; B - \cup (A_1 .. A_n) = \cap((B - A_1) .. (B - A_n)) $$
\begin{equation*}
\begin{aligned}
& \\
& n = 1 \Rightarrow B - (A_1 \cup A_1) = B - A_1 = (B - A_1) \cap (B - A_1) \\
& \\
& n = 2 \Rightarrow B - (A_1 \cup A_2) =  \\
& \qquad \{x \mid x \in B \land x \notin A_1 \land x \notin A_2 \} = \\
& \qquad \{x \mid x \in B \land x \notin A_1 \land 
           x \in B \land x \notin A_2 \} = \\
& \qquad \{x \mid (x \in B \land x \notin A_1) \land 
           (x \in B \land x \notin A_2) \} = \\
& \qquad (B - A_1) \cap (B - A_2) \\
& \\
& n = k + 1 \Rightarrow B - \cup(A_1 .. A_{k+1}) = & (assoc \; \cup) \\
& \qquad B - (\cup(A_1 .. A_k) \cup A_{k+1}) = & (n = 2) \\
& \qquad (B - \cup(A_1 ..A_k)) \cap (B - A_{k+1}) = & (ind. \; hyp.) \\
& \qquad \cap((B - A_1) .. (B - A_k)) \cap (B - A_{k+1}) = & (assoc \; \cap) \\
& \qquad \cap((B - A_1) .. (B - A_{k+1})) \\
& \blacksquare
\end{aligned}
\end{equation*}

\end{document}

