\documentclass[fleqn, 11pt]{article}

\date{January 13, 2020}
\title{Product of presentations of endomaps is presentation of product of endomaps}
\usepackage{amsmath}
\usepackage{amssymb}
\usepackage{mathtools}
\usepackage{tikz-cd}

\begin{document}
\begin{tikzcd}
  P(\alpha)
    \arrow{r}{ \times_p P(\beta) }
    \arrow[xshift = -.7ex, swap]{dd}{ {p_\alpha}^{-1} }
  & P(\alpha \times \beta)
    \arrow[xshift = -.7ex, swap]{dd}{ {p_\beta}^{-1} } \\
  && \\
  \alpha
    \arrow{r}{ \times \beta }
    \arrow[xshift = .7ex, swap]{uu}{ p_\alpha }
    \arrow{r}{ \times \beta }
  & \beta
    \arrow[xshift = .7ex, swap]{uu}{ p_\beta }
\end{tikzcd}

\begin{equation*}
\begin{aligned}
& p_\beta \circ \times \beta = \\
& \qquad p_\beta \circ \times \beta \circ {p_\alpha}^{-1} \circ p_\alpha = \\
& \qquad \times_p P(\beta) \circ p_\alpha \land \\
& p_\alpha \text{ epic } \implies \\
& p_\beta \circ \times \beta \circ {p_\alpha}^{-1} = \times_p P(\beta)
\end{aligned}
\end{equation*}

\hrulefill

$$ \text{ Product of presentation of endomaps is presentation of product of endomaps } $$

\end{document}
